\section{Lecture 24/11/2022}
\noindent\underline{Recap on reflexivity}:

\noindent\(X\) Banach space. \(X^{**} = (X^*)^*\) is the \textbf{bidual space}, \(\mathcal{L}(X^*, \real)\)
\[
    \forall \; x \in X \; \exists \; \Lambda_x : X^* \to \real \mbox{ defined by } \Lambda_x(L) = Lx \quad \forall \; L \in X^*
\]
We proved that \(\Lambda_x \in X^{**}\). Thus we can define the \textbf{canonical map}:
\[
        \begin{array}{lc}
            \tau : & X \to X^{**} \\
            & x \mapsto \Lambda_x
        \end{array}
    \tag*{(Canonical Map)}
\]
We stated that \(\tau\) is an isometric isomorphism from \(X\) into \(\tau(X)\). This is true but for our purpose it's even too much, and it's difficult to prove in details. However, we can prove a slightly weaker result 
\begin{theorem}
    \(\tau\) is linear, continuous, and is an isometry
    \[
        \norm{\tau(x)}_{X^{**}} = \norm{x}_X \quad \forall \; x \in X
    \]
    Moreover, \(\tau\) is injective. If \(\tau\) is also surjective, it is an isometric isomorphism between \(X\) and \(X^{**}\)
\end{theorem}
\begin{proof}
    There are two parts:
    \begin{itemize}
        \item \(\tau\) is linear and continuous: exercise. 
        
        \noindent \(\tau\) is an isometry: \(\norm{\tau(x)}_{X^{**}} = \norm{\Lambda_x}_{X^{**}} = \norm{x}_X\)

        \noindent \(\tau\) is injective: \(x\neq y \Rightarrow \tau(x) \neq \tau(y)\)? 

        \noindent \(x \neq y \Rightarrow\) by the second corollary to Hahn-Banach \(\exists\; L \in X^*\) s.t. \(Lx \neq Ly\).
        \[
            \underset{X^{**}}{\langle}\tau(x), L \underset{X^*}{\rangle} = \Lambda_x(L) = Lx \neq Ly = \Lambda_y(L) = \underset{X^{**}}{\langle}\tau(x), L \underset{X^*}{\rangle}
        \]
        Then, \(\tau(x) \neq \tau(y)\) and \(\tau\) is injective.
        \item Let now \(\tau\) be surjective. Then \(\tau \in \mathcal{L}(x, X^{**})\) and is bijective \(\Rightarrow\) by a corollary of the open map theorem, \(\tau^{-1} \in \mathcal{L}(X^{**}, X)\)
    \end{itemize}
\end{proof}
\begin{definition}
    \(X\) is reflexive if \(\tau\) is surjective. In this case, \(\tau\) is an isometric isomorphism between \(X\) and \(X^{**}\)
\end{definition}

We formally mentioned that
\begin{theorem}
    If \((X, \normdot)\) is uniformly convex \(\Rightarrow\) \((X, \normdot)\) is reflexive.
\end{theorem}

\noindent\textbf{\underline{Remarks}:}
    \begin{proposition}
        If \((X, \normdot)\) is uniformly convex \(\Rightarrow\) \(\overline{B_1(0)}\) is strictly convex.
    \end{proposition}
    \begin{proof}
        Is it true that if \(x, y \in \overline{B_1(0)}\), then \(\frac{x+y}{2} \in B_1(0)\)? Since \((X, \normdot)\) is uniformly convex, we know that \((\norm{x-y}=: \overline{\epsilon}>0)\)
        \[
            \forall \; \overline{\epsilon}>0 \quad \exists \; \overline{\delta} >0 \text{ s.t. } \norm{x} \leq 1 \; \norm{y} \leq \; \norm{x-y} > \frac{\overline{\epsilon}}{2} \Rightarrow \norm{\frac{x+y}{2}} < 1-\overline{delta} 
        \]
        In particular, 
        \[
            \frac{x+y}{2} < 1-\overline{\delta} < 1 \Rightarrow \frac{x+y}{2} \in B_1(0)
        \] 
    \end{proof}
    Consequence: \((\real^2, \normdot_1)\) and \((\real^2, \normdot_\infty)\) are not uniformly convex.
\begin{proposition}
    \((\real^2, \normdot_2)\) is uniformly convex
\end{proposition}
\begin{proof}
    Suppose by contradiction that this is false:
    \( \exists \; \overline{\epsilon} >0 \) and \( \{x_n\}, \{y_n\} \subset \overline{B_1(0)} \) s.t. 
    \[
        \norm{x_n - y_n} > \overline{\epsilon} \text{, but } \norm{\frac{x_n + y_n}{2}} \geq 1 \tag{*}
    \]
    \(\overline{B_1(0)}\) is compact (since we are in \(\real^2\)) \(\Rightarrow\) UTS \(x_n \to \overline{x} \), \(y_n \to \overline{y}\) as \(n \to\infty\). Taking the limit in (*), we deduce that \(\overline{x}\), \(\overline{y} \in \overline{B_1(0)}\)
    \[
        \norm{\overline{x}- \overline{y}} \geq \overline{\epsilon} \text{ , and } \norm{\frac{\overline{x}+\overline{y}}{2}} \geq 1
    \]
    This is not possible, since \(\overline{B_1(0)}\) is strictly convex.
\end{proof}

\begin{theorem}
    \((X, \mathcal{M}, \mu)\) complete measure space. Then \(L^{p}(X)\) is reflexive \(\forall \; p \in (1, \infty)\)
\end{theorem}
\begin{proof}
    \((L^p(X), \normdot_p)\) is uniformly convex \(\forall \; p \in (1, \infty)\) (Clarkson inequalities)
\end{proof}
\(L^1(X) \text{ and } L^\infty(X)\) are not uniformly convex, and not reflexive.

\subsection*{Dual space of \(L^p\)}

\begin{theorem}[Riesz representation theorem]
    \((X, \mathcal{M}, \mu)\) complete measure space, \(p \in (1, \infty)\). Then 
    \[
        \forall\; L \in (L^p(X))^* \quad \exists! \; g \in L^{p'}(X)
    \]
    with \(p' \) conjugate exponent s.t. \(L=L_g\), namely
    \[
        Lf = \int_X fg \, d\mu \qquad \forall\; f \in L^p(X)
    \]
    Moreover \(\norm{L_g}_{(L^p)^*} = \norm{g}_{p'}\)
    
    Thus: \(T: g \in L^{p'} \mapsto L_g \in (L^p)^*\) is an isometric isomorphism.
\end{theorem}
\begin{proof}
    \(1 < p < \infty\). Consider \(T: L^{p'} \to (L^p)^*\) with \(g \mapsto Tg: \langle Tg, f \rangle = \int_X fg \, d\mu\) (namely \(Tg = L_g\)). We already know that
    \[
        \norm{Tg}_* = \norm{L_g}_* = \norm{g}_{p'}
    \]
    \(T\) is injective: for exercise.

    \(T\) is surjective. Indeed, let \(F:= T(L^{p'}) \subseteq (L^p)^*\) subspace. Since \(T\) is an isometry and \(L^{p'}\) is complete, it can be shown that \(T(L^{p'})\) is also complete \(\Rightarrow T(L^{p'})\) is closed.

    If by contradiction \(F \neq (L^p)^*\), then we can apply corollary 3 to Hahn Banach \((X = (L^p)^*), Y=F, x_0 = \lambda\):
    \[
        \exists h \in (L^p)^{**} \text{ s.t. } \langle h, \lambda \rangle \neq 0 \text{ and } h|_F = 0: \langle h, Tg \rangle =0 \quad \forall g \in L^{p'} \tag*{1} 
    \]
    But \(L^p \) is reflexive \((1 <p < \infty)\), then \(h \in L^p \setminus \{0\}\):
    \[
        \langle h, Tg \rangle = (Tg)h = \int_X hg \, d\mu
    \]
    Therefore, (1) tells us that
    \[
        \int_X hg \, d\mu =0 \quad \forall \; g \in L^{p'}(X)
    \]
    Take \(g = \abs{h}^{p-2}h\). Therefore
    \[
        0 = \int_X hg \, d\mu = \int_X h \abs{h}^{p-2} h \, d\mu = \int_X \abs{h}^p \, d\mu \Rightarrow h=0 \in L^p
    \]
    which is the desired contradiction.

    \(T\) is an isomorphism: for exercise.
\end{proof}

\[
    (L^p)^* = L^{p'}
\]

\begin{remark}
    \(p=1\). One can prove the:
\end{remark}
\begin{theorem}
    \((X; \mathcal{M}, \mu)\) complete measure space, \(\sigma\)-finite.
    Then \(\forall\; L \in (L^1(X))^* \quad \exists! \; g \in L^\infty(X)\) s.t. \(L=L_g\):
    \[
        Lf = \int_X fg \, d\mu \quad \forall f \in L^1(X)
    \]
    Moreover, the map \(L \in (L^1)^* \mapsto g \in L^\infty\) is an isometric isomorphism.
\end{theorem}

Recall that \((X, \mathcal{M}, \mu)\) is finite if \(\mu(X) < \infty\).

\begin{definition}
    \((X, \mathcal{M}, \mu)\) is \(\sigma\)-finite if either \(\mu(X) < \infty\), or \(X = \sum_{n=1}^\infty X_n\), where \(\mu(X_n) < \infty\)
\end{definition}

\subsection*{Weak Convergence}

We know that \(\overline{B_1(0)}\) is never compact in \(\infty\) dimension. This is a problem is in proving convergence of sequences. A way to approach this issue consists in weakening the notion of convergence.
\begin{definition}
    \(X\) Banach space. \(\{x_n\} \subset X\) sequence, \(x \in X\). We say that \(x_n\) tends to \(x\) \textbf{weakly} (in \(X\)) as \(n \to \infty\), \(x_n \rightharpoonup x\) in \(X\), if 
    \[
        L x_n \to Lx \qquad \forall \; L \in X^*
    \]
\end{definition}
\begin{remark}
    Assume that \(x_n \to x\) in \(X\), namely \(\norm{x_n -x}_X \to 0\). If \(f:X \to \real\) is continuous, then
    \[
        \lim_{n \to \infty} f(x_n) = f(x)
    \]
    In particular, this is true if \(f = L \in X^*\):
    \[
        \begin{array}{rlc}
            x_n \to x \in X \Rightarrow & L x_n \to Lx & \forall\; L \in X^* \\
            & x_n \rightharpoonup x \in X & \\
            x_n \to x \in X \Rightarrow & x_n \rightharpoonup x \text{ weakly } \in X & \\
             \nLeftarrow & 
        \end{array}
    \]
\end{remark}
\begin{remark}
    We will be interested in weak convergence in \(L^p\). 
    
    \noindent If \(p \in [1, \infty)\), then 
    \[
        f_n \rightharpoonup f \text{ weakly in } L^p(X) \Leftrightarrow \int_X f_n g \, d\mu \to \int_X fg \, d\mu \quad \forall \; g \in L^{p'}
    \]
    \noindent Similarily, in \(l^p = L^P(\natural, \mathcal{P}(\natural), \mu_c)\)
    \[
        x_n \rightharpoonup x \text{ weakly in } l^p \Leftrightarrow \sum_{k=1}^\infty x_n^{(k)} y^{(k)} \to \sum_{k=1}^\infty x^{(k)} y^{(k)} \quad \forall \; y \in l^{p'}
    \]
\end{remark}

\begin{proposition}
    The weak limit is unique (if it exists)
\end{proposition}
\begin{proof}
    By contradiction, suppose that \(\exists \{ x_n\} \subset X\) s.t. \(x_n \rightharpoonup x_1\), \(x_n \rightharpoonup x_2\) weakly in \(X\), \(x_1 \neq x_2\). Then
    \[
        \begin{array}{lc}
            Lx_n \to Lx_1 & \forall\; L \in X^* \\
            Lx_n \to L x_2 & \forall\; L \in X^* \\
            \Rightarrow Lx_1 = Lx_2 & \forall\; L \in X^*
    \end{array} 
    \] 
    By Hahn Banach (corollary 2), this implies \(x_1 = x_2\), a contradiction.
\end{proof}

\begin{proposition}
    If \(x_n \rightharpoonup x\) weakly in \(X\), then \(\{x_n\}\) is bounded, and 
    \[
        \norm{x} \leq \liminf_{n \to \infty} \norm{x_n} \tag*{weak lower semi continuity of \(\normdot\)}
    \]
\end{proposition}
\begin{proof}
    \begin{itemize}
        \item \(\{x_n\}\) is bounded
        
        \(x_n \rightharpoonup x\) weakly \(\Rightarrow \{L x_n\}\) is bounded in \(\real\), \(\forall \; L \in X^*\). Consider \(\Lambda_n \in X^{**}\) def by 
        \[
            \Lambda_n L = L x_n \quad \forall\; L \in X^{*}
        \]
        \(\forall\; L \in X^* \exists\; M_L >0 \) s.t.
        \[
            \abs{\Lambda_n L} = \abs{L x_n } \leq M_L \qquad \forall\; n \tag*{PB}
        \]
        (pointwise boundedness of \(\{\Lambda_n \} \subset X^{**}\))
        \[
            \Lambda_n: X^{*}= \mathcal{L}(X, \real) \to \real    
        \]
        By Banach Steinhaus, \(\{\Lambda_n\}\) is uniformly bounded:
        \[
            \sup_n \norm{ \Lambda_n}_{\mathcal{L}(X^*, \real)} \leq M
        \]
        Moreover, by Hahn Banach, \(\forall \; n \in \natural \quad \exists L_n \in X^*\) s.t. \(\norm{L_n}_* = 1 \) and \(L_n x_n = \norm{x_n}\). Therefore
        \[
            \norm{x_n} = \abs{L_n x_n} = \abs{\Lambda_n L_n} \leq \norm{\Lambda_n}_\mathcal{L} \norm{L_n}_* \leq M \quad \forall n \in \natural
        \] 
        \item \(x_n \rightharpoonup x\) weakly. 
        
        By corollary 1 of Hahn Banach, \(\exists L_x \in x^*\) s.t. \(\norm{L_x}_* = 1\) and \(L_x x = \norm{x}\). Then
        \[
            \norm{x} = \abs{L_x x} = \lim_n \abs{L_x x_n} = \liminf_n \abs{L_x x_n} \leq \liminf_n \norm{L_x}_* \norm{x_n }_X = \liminf_n \norm{x_n }_X
        \]    
    \end{itemize}
\end{proof}

\begin{proposition}
    \(x_n \rightharpoonup x \) in \(X\) weakly, and \(L_n \to L\) (strongly) in \(X^*\). Then
    \[
        L_n x_n \to Lx \quad \text{ in } \real
    \]
\end{proposition}
\begin{proposition}
    \(X, Y\) Banach, \(T \in \mathcal{L}(X, Y)\)
    \[
        x_n \rightharpoonup x \text{ weakly } \Rightarrow Tx_n \rightharpoonup Tx \text{ weakly }
    \]
\end{proposition}